src/mcl/lemmas.lean
@@ -1,0 +1,25 @@
+import mcl.defs
+import mcl.rhl
+
+open parlang
+open mcl
+open mcl.rhl
+open parlang.thread_state
+
+@[simp]
+lemma store_stores {sig : signature} {dim} {idx : vector (expression sig type.int) dim} {var t} {h₁ : type_of (sig.val var) = t} {h₂}
+{ts : thread_state (memory $ parlang_mcl_tlocal sig) (parlang_mcl_global sig)} {i : mcl_address sig} : 
+i ∉ (mcl_store var idx h₁ h₂ ts).stores → i ∉ ts.stores := by simp [mcl_store, store, not_or_distrib]
+
+@[simp]
+lemma store_loads {sig : signature} {dim} {idx : vector (expression sig type.int) dim} {var t} {h₁ : type_of (sig.val var) = t} {h₂}
+{ts : thread_state (memory $ parlang_mcl_tlocal sig) (parlang_mcl_global sig)} {i : mcl_address sig} : 
+i ∉ (mcl_store var idx h₁ h₂ ts).loads → i ∉ ts.loads := by simp [mcl_store, store, not_or_distrib]
+
+@[simp]
+lemma array_hole_name_neq {sig : signature} (var₁ var₂ : string) (h : var₁ ≠ var₂) (idx : vector ℕ (((sig.val var₁).type).dim)) :
+(⟨var₁, idx⟩ : mcl_address sig) ∉ @array_address_range sig var₂ := begin
+    unfold array_address_range,
+    intro,
+    contradiction,
+end
